Dependency Work upload

src/coq/Dependency/DataDependency.v
@@ -5,6 +5,9 @@ Require Import Bool.
 Require Import Coq.Strings.String.
 Require Import Coq.Arith.EqNat.
 
+Require Import Vellvm.Util.
+Require Import Vellvm.Dependency.DEPIMP Vellvm.Dependency.SetTheory.
+
 From mathcomp.ssreflect
 Require Import ssreflect ssrbool fingraph fintype path
   ssrfun eqtype
@@ -13,340 +16,97 @@ Require Import ssreflect ssrbool fingraph fintype path
 
 
 
+(** Calculating Memory Read in a given expression**)
 
-(*Util + Maps*)
-Inductive id : Type :=
-  | Id : nat -> id.
-
-Definition total_map (A:Type) := id -> A.
-
-Definition state := total_map nat.
-
-
-
-Fixpoint beq_nat (n m : nat) : bool :=
-  match n with
-  | O => match m with
-         | O => true
-         | S m' => false
-         end
-  | S n' => match m with
-            | O => false
-            | S m' => beq_nat n' m'
-            end
-  end.
-
-
-Definition beq_id id1 id2 :=
-  match (id1, id2) with
-    (Id n1, Id n2) => beq_nat n1 n2
-  end.
-
-
-Definition t_update {A:Type} (m : total_map A)
-                    (x : id) (v : A) :=
-  fun x' => if beq_id x x' then v else m x'.
-
-
-Definition t_empty {A:Type} (v : A) : total_map A :=
-  (fun _ => v).
-
-
-Definition empty_state : state :=
-  t_empty 0.
-
-
-
-
-
-
-Fixpoint leb (n m : nat) : bool :=
-  match n with
-  | O => true
-  | S n' =>
-      match m with
-      | O => false
-      | S m' => leb n' m'
-      end
-  end.
-
-
-
-(*IMP*)
-
-
-
-Inductive aexp : Type :=
-  | ANum : nat -> aexp
-  | AId : id -> aexp
-  | APlus : aexp -> aexp -> aexp
-  | AMinus : aexp -> aexp -> aexp
-  | AMult : aexp -> aexp -> aexp.
-
-
-Inductive bexp : Type :=
-  | BTrue : bexp
-  | BFalse : bexp
-  | BEq : aexp -> aexp -> bexp
-  | BLe : aexp -> aexp -> bexp
-  | BNot : bexp -> bexp
-  | BAnd : bexp -> bexp -> bexp.
-
-
-Inductive com : Type :=
-  | CAss : id -> aexp -> com
-  | CIf : bexp -> com -> com -> com
-  | CWhile : bexp -> com -> com.
-
-
-
-
-Fixpoint aeval (st : state) (a : aexp) : nat :=
+Fixpoint singleAexpRead (a:aexp) :=
   match a with
-  | ANum n => n
-  | AId x => st x                                (* <----- NEW *)
-  | APlus a1 a2 => (aeval st a1) + (aeval st a2)
-  | AMinus a1 a2  => (aeval st a1) - (aeval st a2)
-  | AMult a1 a2 => (aeval st a1) * (aeval st a2)
-  end.
-
-Fixpoint beval (st : state) (b : bexp) : bool :=
-  match b with
-  | BTrue       => true
-  | BFalse      => false
-  | BEq a1 a2   => beq_nat (aeval st a1) (aeval st a2)
-  | BLe a1 a2   => leb (aeval st a1) (aeval st a2)
-  | BNot b1     => negb (beval st b1)
-  | BAnd b1 b2  => andb (beval st b1) (beval st b2)
-  end.
-
-
-Reserved Notation "c1 '/' st '\\' st'"
-                  (at level 40, st at level 39).
-
-
-Notation "x '::=' a" :=
-  (CAss x a) (at level 60).
-Notation "'WHILE' b 'DO' c 'END'" :=
-  (CWhile b c) (at level 80, right associativity).
-Notation "'IFB' c1 'THEN' c2 'ELSE' c3 'FI'" :=
-  (CIf c1 c2 c3) (at level 80, right associativity).
-
-
-
-Inductive ceval : com -> state -> state -> Prop :=
-  | E_Ass  : forall st a1 n x,
-      aeval st a1 = n ->
-      (x ::= a1) / st \\ (t_update st x n)
-  | E_IfTrue : forall st st' b c1 c2,
-      beval st b = true ->
-      c1 / st \\ st' ->
-      (IFB b THEN c1 ELSE c2 FI) / st \\ st'
-  | E_IfFalse : forall st st' b c1 c2,
-      beval st b = false ->
-      c2 / st \\ st' ->
-      (IFB b THEN c1 ELSE c2 FI) / st \\ st'
-  | E_WhileEnd : forall b st c,
-      beval st b = false ->
-      (WHILE b DO c END) / st \\ st
-  | E_WhileLoop : forall st st' st'' b c,
-      beval st b = true ->
-      c / st \\ st' ->
-      (WHILE b DO c END) / st' \\ st'' ->
-      (WHILE b DO c END) / st \\ st''
-
-  where "c1 '/' st '\\' st'" := (ceval c1 st st').
-
-
-(*********************************************************************************)
-
-
-(*Get all the previous instructions*)
-
-Inductive instruction :=
-  | ins (v:com) (a:nat).
-
-
-
-Variable (l: seq instruction).
-
-
-
-Definition equalInstruction (b:instruction) (a:instruction) :=
-  match b,a with
-  | (ins _ c), (ins _ d) => (beq_nat c d)
+  | ANum _ => nil
+  | AId b => b :: nil
+  | APlus b c => singleAexpRead b ++ singleAexpRead c
+  | AMult b c => singleAexpRead b ++ singleAexpRead c
+  | AMinus b c => singleAexpRead b ++ singleAexpRead c
 end.
 
 
-
-
-Check find.
-
-(* Get a list of all the previous instructions *)
-Definition getInstructionList (b:instruction) := 
-  let i := find (equalInstruction b) l in
-  match i with
-  | 0 => None
-  | a.+1 => Some (drop a l)
-end.
-
-
-(*
-Fixpoint checkAssignment (c:com) (i:id) :=
+Fixpoint singleBexpRead (c:bexp) :=
   match c with
-  | CIf a b c => checkAssignment c i
-  | CWhile a b => checkAssignment b i
-  | CAss a b => if beq_nat a i then 1 else 0
-end.
-*)
-
-
-
-
-
-
-
-Fixpoint checkRead (a:aexp) (i:id) :=
-  match a with
-  | ANum _ => 0
-  | AId b => if b = i then 1 else 0
-  | APlus c b => checkRead c i + checkRead b i
-  | AMinus c b => checkRead c i + checkRead b i
-  | AMult c b => checkRead c i + checkRead b i
+  | BTrue => nil
+  | BFalse => nil
+  | BEq a b => singleAexpRead b ++ singleAexpRead a
+  | BLe a b => singleAexpRead b ++ singleAexpRead a
+  | BNot _ => nil
+  | BAnd a b => singleBexpRead b ++ singleBexpRead a
 end.
 
 
 
 
-
-
-
-
-
-
-
-
-
-
-
-
-
-
-
-
-
-
-
-
-
-
-
-
-
-
-
-
-
-
-(*********************************************************************)
-(*SCRAP IDEAS*)
-(*********************************************************************)
-
-Inductive variable :=
-  | A
-  | B
-  | C
-  | const (cs:nat).
-
-
-Inductive dependency :=
-  | Dep (v:variable) (a:nat) (b:nat).
-
-
-Inductive state :=
-  | st (v:variable) (a:nat).
-
-
-Variable (l: seq dependency).
-Variable (s: list state).
-
-
-
-Definition equalVar (a b: variable) :=
-  match a, b with
-  | A, A => true
-  | B, B => true
-  | C, C => true
-  | _, _ => false
+Fixpoint sMR (c:com) :=
+  match c with
+  | CAss a b => singleAexpRead b (**need to check*)
+  | CIf a b c => singleBexpRead a ++ sMR b ++ sMR c
+  | CWhile a b => singleBexpRead a ++ sMR b
+  | CSkip => nil
+  | CSeq a b => sMR a ++ sMR b
+  | CFor a b c d => sMR d (*done*)
+  | CFrom a b c => sMR c
 end.
 
 
 
-Definition equalDep (b:variable) (a : dependency) :=
-  match a with
-  | (Dep c _ _) => equalVar b c
-end.
+(** Calculating Memory Written in a given expression **)
 
 
-Definition equalState (b:variable) (a:state) :=
-  match a with
-  | (st a _) => equalVar a b
-end.
-
-
-Definition findDep (b:variable) := find (equalDep b) l.
-
-Definition findVarState (b:variable) := find (equalState b) s.
-
-
-Fixpoint getItem (A:Type) (l:list A) (n:nat) :=
-  match l, n with
-  | nil,_  => None
-  | (a::s), 0 => Some a
-  | (a::s), b.+1 => getItem A s b
-end.
-
-
-Print find.
-
-
-
-
-
-Definition retrieveVar (b:variable) :=
-  let vr := findVarState b in
-  match vr with
-  | 0 => None
-  | a.+1 => let x := getItem state s a in
-            match x with
-            | None => None
-            | Some (st d e) => Some e
-            end
+Fixpoint sMW (c:com) :=
+  match c with
+  | CAss a _ => a :: nil (**need to check*)
+  | CIf _ b c => sMW b ++ sMW c
+  | CWhile _ b => sMW b
+  | CSeq a b => sMW a ++ sMW b
+  | CSkip => nil
+  | CFor a b c d => a :: sMW d
+  | CFrom a b c => sMW c
 end.
 
 
 
-Definition setVariable (b:variable) (n:nat) := 0.
+Definition cequiv (c1 c2 : com) : Prop :=
+  forall (st st' : state),
+    (c1 / st \\ st') <-> (c2 / st \\ st').
 
 
 
 
 
 
+Definition no_data_dependency_calc (a b: com) : bool := nilp ((sMR a u sMW b) n (sMW a u sMR b) n (sMW a u sMW b)).
 
 
+Definition sampleSingleLineProgram := CAss W (APlus (ANum 1) (ANum 1)).
+Definition sampleSingleLineProgram1 := CAss X (APlus (AId W) (AId W)).
+Definition sampleSingleLineProgram2 := CAss Y (AMinus (AId W) (ANum 1)).
+Definition sampleSingleLineProgram3 := CAss Z (AMult (AId Y) (ANum 5)).
+Definition sampleSingleLineProgram4 := CAss W (APlus (AMinus (AId Z) (ANum 1)) (AId X)).
 
 
-
-Inductive instruction :=
-  | Add (pc:nat) (v1:variable) (v2:variable) (v3:variable)
-.
-
-
-Check foldr.
+Eval compute in no_data_dependency_calc sampleSingleLineProgram sampleSingleLineProgram1.
+Eval compute in no_data_dependency_calc sampleSingleLineProgram1 sampleSingleLineProgram2.
+Eval compute in no_data_dependency_calc sampleSingleLineProgram1 sampleSingleLineProgram3.
 
 
+Fixpoint DataDependencyInCommands (c: com) :=
+  match c with
+  | CSeq a b => (no_data_dependency_calc a b) || DataDependencyInCommands b
+  | CIf _ a b => DataDependencyInCommands a || DataDependencyInCommands b 
+  | CWhile _ _ => false
+  | CAss _ _ => false
+  | CFrom _ _ a => DataDependencyInCommands a
+  | CFor _ _ _ a => DataDependencyInCommands a
+  | CSkip => false
+end.
 
-Variable (V: nat)(E: Type)(r: seq instruction).
-Definition sum := foldr countAinV1 0 r.
-(*c
+
+Theorem test : forall a, cequiv (a) (CFrom 0 1 a).
+Proof. split;intros.
+-inversion H; subst.
+  +apply E_FromEnd.
